2021/day24/README.md
@@ -1,0 +1,59 @@
+# Day 24 solution notes
+
+I decided I wanted to take a decompilation or symbolic execution approach,
+even though it was probably not the most efficient.  The advantage is
+that I could more easily prove correctness of each reduction, and avoid
+doing brute-force search.  Which I hoped would be useful for part 2.
+
+Eventually I realized that what I wanted was to build a tree of conditionals
+which would allow case-by-case analysis.  So the symbolic execution attempt
+to preserve a "normal form" which consists of `IfEqThen` operations
+with non-conditional expressions at the leaves, and no conditionals
+appearing in the values being tested for equality.
+
+The final piece was writing two cases to eliminate impossible conditions, which dramatically
+reduced the number of possibilities: down to 1!
+
+```
+(+ i_2 -1 )  == i_3  /\
+(+ i_4 5 )  == i_5  /\
+(+ i_6 8 )  == i_7  /\
+(+ i_1 4 )  == i_8  /\
+(+ (% (+ i_0 7 ) 26 ) -4 )  == i_9  /\
+(+ i_11 -6 )  == i_12  /\
+(+ (% (+ i_10 12 ) 26 ) -10 )  == i_13 
+```
+
+That meant I didn't have to write the code to numerically compare different possibilities.
+(I went back and did this last step only after previous output showed a lot of conditions
+that were impossible.)
+
+I successfully proved all the transformations correct!
+
+I did not do the same for the search procedure.  I eventually just resorted to
+brute-force search because layering an SMT solver on top of F* was not something I wanted
+to do.  :)  But, it would be nice to see what sort of thing we could do to make
+the solver more efficient.
+
+## F* successes
+
+Pattern matching FTW.
+
+I couldn't prove a + (b % m) = (a+b) %m because it wasn't true!  Oops.
+
+Similarly, I couldn't prove that my bounds check for the case of `(+ (% (+ i_a k) 26) y) == i_b` was
+correct, because it had a bug! I thought it was just a problem of not having the modulus lemmas.
+
+## F* problems
+
+Can't match on a negative integer, because it's not treated as a literal
+by the parser: https://github.com/FStarLang/FStar/issues/2415
+
+It sure would be nice if the F* standard library had ways to print lists by default.
+
+## Questions
+
+I was only able to prove `push_op_correctness` for `AddOp`.  Taking a general function of type
+`expr->expr->expr` seems very hard to reason about.  I tried writing a condition I thought would
+be sufficient but the same problem occurred.  I don't know what the correct type to use here is;
+can we define a sufficiently well-behaved condition that all the constructors have?
